test: extend inductive_pred.lean with tests using the new construction.

tests/lean/run/inductive_pred.lean
@@ -2,6 +2,12 @@ namespace Ex
 inductive LE : Nat → Nat → Prop
   | refl : LE n n
   | succ : LE n m → LE n m.succ
+  
+def typeOf {α : Sort u} (a : α) := α 
+
+theorem LE_brecOn : typeOf @LE.brecOn = 
+∀ {motive : (a a_1 : Nat) → LE a a_1 → Prop} {a a_1 : Nat} (x : LE a a_1),
+  (∀ (a a_2 : Nat) (x : LE a a_2), @LEProofBelow motive a a_2 x → motive a a_2 x) → motive a a_1 x := rfl
 
 theorem LE.trans : LE m n → LE n o → LE m o := by
   intro h1 h2
@@ -16,6 +22,9 @@ theorem LE.trans' : LE m n → LE n o → LE m o
 inductive Even : Nat → Prop
   | zero : Even 0
   | ss   : Even n → Even n.succ.succ
+
+theorem Even_brecOn : typeOf @Even.brecOn = ∀ {motive : (a : Nat) → Even a → Prop} {a : Nat} (x : Even a),
+  (∀ (a : Nat) (x : Even a), @EvenProofBelow motive a x → motive a x) → motive a x := rfl
 
 theorem Even.add : Even n → Even m → Even (n+m) := by
   intro h1 h2
@@ -33,6 +42,9 @@ theorem mul_left_comm (n m o : Nat) : n * (m * o) = m * (n * o) := by
 inductive Power2 : Nat → Prop
   | base : Power2 1
   | ind  : Power2 n → Power2 (2*n) -- Note that index here is not a constructor
+  
+theorem Power2_brecOn : typeOf @Power2.brecOn = ∀ {motive : (a : Nat) → Power2 a → Prop} {a : Nat} (x : Power2 a),
+  (∀ (a : Nat) (x : Power2 a), @Power2ProofBelow motive a x → motive a x) → motive a x := rfl
 
 theorem Power2.mul : Power2 n → Power2 m → Power2 (n*m) := by
   intro h1 h2
@@ -45,4 +57,64 @@ theorem Power2.mul : Power2 n → Power2 m → Power2 (n*m) := by
 -- theorem Power2.mul' : Power2 n → Power2 m → Power2 (n*m)
 --  | h1, base => by simp_all
 --  | h1, ind h2 => mul_left_comm .. ▸ ind (mul' h1 h2)
+
+inductive tm : Type :=
+  | C : Nat → tm 
+  | P : tm → tm → tm
+
+open tm
+
+set_option hygiene false in
+infixl:40 " ==> " => step
+inductive step : tm → tm → Prop :=
+  | ST_PlusConstConst : ∀ n1 n2,
+      P (C n1) (C n2) ==> C (n1 + n2)
+  | ST_Plus1 : ∀ t1 t1' t2,
+      t1 ==> t1' →
+      P t1 t2 ==> P t1' t2
+  | ST_Plus2 : ∀ n1 t2 t2',
+      t2 ==> t2' →
+      P (C n1) t2 ==> P (C n1) t2'
+
+def deterministic {X : Type} (R : X → X → Prop) :=
+  ∀ x y1 y2 : X, R x y1 → R x y2 → y1 = y2
+
+theorem step_deterministic' : deterministic step := λ x y₁ y₂ hy₁ hy₂ => 
+  @step.brecOn (λ s t st => ∀ y₂, s ==> y₂ → t = y₂) _ _ hy₁ (λ s t st hy₁ y₂ hy₂ => 
+    match hy₁, hy₂ with
+    | stepProofBelow.ST_PlusConstConst _ _, step.ST_PlusConstConst _ _ => rfl
+    | stepProofBelow.ST_Plus1 _ _ _ _ hy₁ ih, step.ST_Plus1 _ t₁' _ _ => by rw ←ih t₁'; assumption
+    | stepProofBelow.ST_Plus1 _ _ _ _ hy₁ ih, step.ST_Plus2 _ _ _ _ => by cases hy₁
+    | stepProofBelow.ST_Plus2 _ _ _ _ _ ih, step.ST_Plus2 _ _ t₂ _ => by rw ←ih t₂; assumption
+    | stepProofBelow.ST_Plus2 _ _ _ _ hy₁ _, step.ST_PlusConstConst _ _ => by cases hy₁
+    ) y₂ hy₂ 
+
+section NestedRecursion
+
+axiom f : Nat → Nat
+
+inductive is_nat : Nat -> Prop
+| Z : is_nat 0
+| S {n} : is_nat n → is_nat (f n)
+
+axiom P : Nat → Prop
+axiom F0 : P 0
+axiom F1 : P (f 0)
+axiom FS {n : Nat} : P n → P (f (f n))
+
+-- we would like to write this
+-- theorem foo : ∀ {n}, is_nat n → P n
+-- | _, is_nat.Z => F0
+-- | _, is_nat.S is_nat.Z => F1
+-- | _, is_nat.S (@is_nat.S n h) => FS (foo h)
+
+theorem foo' : ∀ {n}, is_nat n → P n := fun h => 
+  @is_nat.brecOn (fun n hn => P n) _ h fun n h ih => 
+  match ih with
+  | is_natProofBelow.Z => F0 
+  | is_natProofBelow.S _ is_natProofBelow.Z _ => F1
+  | is_natProofBelow.S _ (is_natProofBelow.S a b hx) h₂ => FS hx
+
+end NestedRecursion
+
 end Ex
